more proof

Given_Clause_Loops/Fair_DISCOUNT_Loop.thy
@@ -13,6 +13,11 @@ theory Fair_DISCOUNT_Loop
 begin
 
 
+subsection \<open>Setup\<close>
+
+hide_const (open) Seq.chain
+
+
 section \<open>Locale\<close>
 
 type_synonym ('p, 'f) fair_DL_state = "'p \<times> 'f option \<times> 'f fset"
@@ -74,6 +79,12 @@ definition passive_inferences_of :: "'p \<Rightarrow> 'f inference set" where
 definition passive_formulas_of :: "'p \<Rightarrow> 'f set" where
   "passive_formulas_of P = {C. Passive_Formula C \<in> elems P}"
 
+lemma passive_inferences_of[simp]: "passive_inferences_of empty = {}"
+  unfolding passive_inferences_of_def by simp
+
+lemma passive_formulas_of[simp]: "passive_formulas_of empty = {}"
+  unfolding passive_formulas_of_def by simp
+
 fun fstate :: "'p \<times> 'f option \<times> 'f fset \<Rightarrow> 'f inference set \<times> ('f \<times> DL_label) set" where
   "fstate (P, Y, A) = state (passive_inferences_of P, passive_formulas_of P, set_option Y, fset A)"
 
@@ -112,7 +123,10 @@ fun formulas_union :: "'f set \<times> 'f set \<times> 'f set \<Rightarrow> 'f s
 inductive
   fair_DL :: "('p, 'f) fair_DL_state \<Rightarrow> ('p, 'f) fair_DL_state \<Rightarrow> bool" (infix "\<leadsto>DLf" 50)
 where
-  choose_p: "P \<noteq> empty \<Longrightarrow> select P = Passive_Formula C \<Longrightarrow>
+  compute_infer: "P \<noteq> empty \<Longrightarrow> select P = Passive_Inference \<iota> \<Longrightarrow>
+    \<iota> \<in> no_labels.Red_I (fset A \<union> {C}) \<Longrightarrow>
+    (P, None, A) \<leadsto>DLf (remove (select P) P, Some C, A)"
+| choose_p: "P \<noteq> empty \<Longrightarrow> select P = Passive_Formula C \<Longrightarrow>
     (P, None, A) \<leadsto>DLf (remove (select P) P, Some C, A)"
 | delete_fwd: "C \<in> no_labels.Red_F (fset A) \<or> (\<exists>C' \<in> fset A. C' \<preceq>\<cdot> C) \<Longrightarrow>
     (P, Some C, A) \<leadsto>DLf (P, None, A)"
@@ -122,13 +136,159 @@ where
     (P, Some C, A |\<union>| {|C'|}) \<leadsto>DLf (P, Some C, A)"
 | simplify_bwd: "C'' \<prec>S C' \<Longrightarrow> C' \<in> no_labels.Red_F {C, C''} \<Longrightarrow>
     (P, Some C, A |\<union>| {|C'|}) \<leadsto>DLf (add (Passive_Formula C'') P, Some C, A)"
-| compute_infer: "P \<noteq> empty \<Longrightarrow> select P = Passive_Inference \<iota> \<Longrightarrow>
-    \<iota> \<in> no_labels.Red_I (fset A \<union> {C}) \<Longrightarrow>
-    (P, None, A) \<leadsto>DLf (remove (select P) P, Some C, A)"
 | schedule_infer: "set \<iota>s = no_labels.Inf_between (fset A) {C} \<Longrightarrow>
     (P, Some C, A) \<leadsto>DLf (fold (add \<circ> Passive_Inference) \<iota>s P, None, A |\<union>| {|C|})"
-| delete_orphan_formulas: "set \<iota>s \<inter> no_labels.Inf_from (fset A) = {} \<Longrightarrow>
+| delete_orphan_formulas: "\<iota>s \<noteq> [] \<Longrightarrow> set \<iota>s \<subseteq> passive_inferences_of P \<Longrightarrow>
+    set \<iota>s \<inter> no_labels.Inf_from (fset A) = {} \<Longrightarrow>
     (P, Y, A) \<leadsto>DLf (fold (remove \<circ> Passive_Inference) \<iota>s P, Y, A)"
+
+
+subsection \<open>Initial State\<close>
+
+inductive is_initial_fair_DL_state :: "('p, 'f) fair_DL_state \<Rightarrow> bool" where
+  "passive_inferences_of P = {\<iota> \<in> Inf_F. prems_of \<iota> = []} \<Longrightarrow>
+   is_initial_fair_DL_state (P, None, {||})"
+
+
+subsection \<open>Invariant\<close>
+
+inductive fair_DL_invariant :: "('p, 'f) fair_DL_state \<Rightarrow> bool" where
+  "passive_inferences_of P \<subseteq> Inf_F \<Longrightarrow> fair_DL_invariant (P, Y, A)"
+
+lemma initial_fair_DL_invariant: "is_initial_fair_DL_state St \<Longrightarrow> fair_DL_invariant St"
+  unfolding is_initial_fair_DL_state.simps fair_DL_invariant.simps by auto
+
+lemma step_fair_DL_invariant:
+  assumes
+    inv: "fair_DL_invariant St" and
+    step: "St \<leadsto>DLf St'"
+  shows "fair_DL_invariant St'"
+  using step inv apply cases
+  apply (simp_all add: fair_DL_invariant.intros)
+
+lemma chain_fair_DL_invariant_lnth:
+  assumes
+    chain: "chain (\<leadsto>DLf) Sts" and
+    fair_hd: "fair_DL_invariant (lhd Sts)" and
+    i_lt: "enat i < llength Sts"
+  shows "fair_DL_invariant (lnth Sts i)"
+  using i_lt
+proof (induct i)
+  case 0
+  thus ?case
+    using fair_hd lhd_conv_lnth zero_enat_def by fastforce
+next
+  case (Suc i)
+  thus ?case
+    using chain step_fair_DL_invariant
+    by (metis dual_order.refl fair_DL_invariant.intros fstate.cases)
+qed
+
+lemma chain_fair_DL_invariant_llast:
+  assumes
+    chain: "chain (\<leadsto>DLf) Sts" and
+    fair_hd: "fair_DL_invariant (lhd Sts)" and
+    fin: "lfinite Sts"
+  shows "fair_DL_invariant (llast Sts)"
+proof -
+  obtain i :: nat where
+    i: "llength Sts = enat i"
+    using lfinite_llength_enat[OF fin] by blast
+
+  have im1_lt: "enat (i - 1) < llength Sts"
+    using i by (metis chain chain_length_pos diff_less enat_ord_simps(2) less_numeral_extra(1)
+        zero_enat_def)
+
+  show ?thesis
+    using chain_fair_DL_invariant_lnth[OF chain fair_hd im1_lt]
+    by (metis Suc_diff_1 chain chain_length_pos eSuc_enat enat_ord_simps(2) i llast_conv_lnth
+        zero_enat_def)
+qed
+
+
+subsection \<open>Final State\<close>
+
+inductive is_final_fair_DL_state :: "('p, 'f) fair_DL_state \<Rightarrow> bool" where
+  "is_final_fair_DL_state (empty, None, A)"
+
+lemma is_final_fair_DL_state_iff_no_DLf_step:
+  assumes inv: "fair_DL_invariant St"
+  shows "is_final_fair_DL_state St \<longleftrightarrow> (\<forall>St'. \<not> St \<leadsto>DLf St')"
+proof
+  assume "is_final_fair_DL_state St"
+  then obtain A :: "'f fset" where
+    st: "St = (empty, None, A)"
+    by (auto simp: is_final_fair_DL_state.simps)
+  show "\<forall>St'. \<not> St \<leadsto>DLf St'"
+    unfolding st
+  proof (intro allI notI)
+    fix St'
+    assume "(empty, None, A) \<leadsto>DLf St'"
+    thus False
+      by cases auto
+  qed
+next
+  assume no_step: "\<forall>St'. \<not> St \<leadsto>DLf St'"
+  show "is_final_fair_DL_state St"
+  proof (rule ccontr)
+    assume not_fin: "\<not> is_final_fair_DL_state St"
+
+    obtain P :: 'p and Y :: "'f option" and A :: "'f fset" where
+      st: "St = (P, Y, A)"
+      by (cases St)
+
+    have "P \<noteq> empty \<or> Y \<noteq> None"
+      using not_fin unfolding st is_final_fair_DL_state.simps by auto
+    moreover {
+      assume
+        p: "P \<noteq> empty" and
+        y: "Y = None"
+
+      have "\<exists>St'. St \<leadsto>DLf St'"
+      proof (cases "select P")
+        case sel: (Passive_Inference \<iota>)
+        hence \<iota>_inf: "\<iota> \<in> Inf_F"
+          using inv p unfolding st by (metis fair_DL_invariant.cases fst_conv mem_Collect_eq
+              passive_inferences_of_def select_in_elems subset_iff)
+        have \<iota>_red: "\<iota> \<in> no_labels.Red_I_\<G> (fset A \<union> {concl_of \<iota>})"
+          using \<iota>_inf no_labels.empty_ord.Red_I_of_Inf_to_N by auto
+        show ?thesis
+          using fair_DL.compute_infer[OF p sel \<iota>_red] unfolding st p y by blast
+      next
+        case (Passive_Formula C)
+        then show ?thesis
+          using fair_DL.choose_p[OF p] unfolding st p y by fast
+      qed
+    } moreover {
+      assume "Y \<noteq> None"
+      then obtain C :: 'f where
+        y: "Y = Some C"
+        by blast
+
+      have n: "N = {||}" and
+        x: "X = None"
+        using y inv' by blast+
+
+      let ?M = "concl_of ` no_labels.Inf_between (fset A) {C}"
+
+      have fin: "finite ?M"
+        by (simp add: finite_Inf_between)
+      have fset_abs_m: "fset (Abs_fset ?M) = ?M"
+        by (rule Abs_fset_inverse[simplified, OF fin])
+
+      have inf_red: "no_labels.Inf_between (fset A) {C}
+        \<subseteq> no_labels.Red_I_\<G> (fset A \<union> {C} \<union> fset (Abs_fset ?M))"
+        by (simp add: fset_abs_m no_labels.Inf_if_Inf_between no_labels.empty_ord.Red_I_of_Inf_to_N
+            subsetI)
+
+      have "\<exists>St'. St \<leadsto>DLf St'"
+        using fair_DL.infer[OF inf_red] unfolding st n x y by fast
+    } ultimately show False
+      using no_step by force
+  qed
+qed
+
+
 
 end
 
